HepLean/Lorentz/ComplexTensor/PauliMatrices/CoContractContr.lean
@@ -4,7 +4,6 @@ Released under Apache 2.0 license as described in the file LICENSE.
 Authors: Joseph Tooby-Smith
 -/
 import HepLean.Lorentz.ComplexTensor.PauliMatrices.Basis
-import HepLean.Lorentz.ComplexTensor.Lemmas
 /-!
 
 ## Contractiong of indices of Pauli matrix.
